lib/zoo_parabs/vertex.mli
@@ -1,17 +1,21 @@
 type t
 
+type task =
+  unit Pool.task
+
 val create :
-  bool Pool.task option -> t
+  task option -> t
 
 val task :
-  t -> bool Pool.task
+  t -> task
 val set_task :
-  t -> bool Pool.task -> unit
-val set_task' :
-  t -> unit Pool.task -> unit
+  t -> task -> unit
 
 val precede :
   t -> t -> unit
 
 val release :
   Pool.context -> t -> unit
+
+val yield :
+  Pool.context -> t -> task -> unit
