theories/zoo_parabs/vertex__opaque.v
@@ -4,6 +4,6 @@ From zoo_parabs Require Import
 #[global] Opaque vertex_create.
 #[global] Opaque vertex_task.
 #[global] Opaque vertex_set_task.
-#[global] Opaque vertex_set_task'.
 #[global] Opaque vertex_precede.
 #[global] Opaque vertex_release.
+#[global] Opaque vertex_yield.
